src/SingleValueSyn.v
@@ -22,6 +22,30 @@ Section Impl.
   Local Definition impl0 := impl0 extIdx1 extIdx2.
   Local Definition svmP := svmP extIdx1 extIdx2.
 
+  Lemma svmMsgF_ValidMsgMap:
+    ValidMsgMap (svmMsgF extIdx1 extIdx2) impl0 spec.
+  Proof.
+    unfold ValidMsgMap; intros.
+    unfold svmMsgF; simpl.
+    unfold svmIdxF, isInternal.
+    unfold impl0.
+    split.
+    - find_if_inside.
+      + reflexivity.
+      + find_if_inside; auto.
+        elim n; clear n.
+        Common.dest_in.
+        rewrite <-H.
+        simpl; tauto.
+    - find_if_inside.
+      + reflexivity.
+      + find_if_inside; auto.
+        elim n; clear n.
+        Common.dest_in.
+        rewrite <-H.
+        simpl; tauto.
+  Qed.
+
   (** First, prove that the initial system is provided properly. *)
   Theorem impl0_ok: SynthOk spec (SimTrs SvmR) svmP impl0.
   Proof.
@@ -34,30 +58,21 @@ Section Impl.
   
   Section SynStep.
 
-    Local Definition targetObjIdx := child1Idx.
-    Local Definition targetTrsIdx := 0.
-
-    Ltac get_target_trs impl oidx tidx :=
+    Ltac get_target_trs impl oidx tidx pname :=
       let oobj := (eval cbn in (nth_error (sys_objs impl) oidx)) in
       match oobj with
       | Some ?obj =>
         let otrs := (eval cbn in (nth_error (obj_trs obj) tidx)) in
         match otrs with
-        | Some ?trs => exact trs
+        | Some ?trs => pose trs as pname
         end
       end.
 
-    Ltac cbner t := let ct := (eval cbn in t) in exact ct.
+    Ltac cbner t tn := let ct := (eval cbn in t) in pose ct as tn.
+    Ltac hnfer t tn := let ht := (eval hnf in t) in pose ht as tn.
 
-    Ltac get_precond trs :=
-      cbner (pmsg_precond trs).
-    
-    Local Definition targetTrs: PMsg :=
-      ltac:(get_target_trs impl0 targetObjIdx targetTrsIdx).
-
-    Local Definition targetMid: MsgId := pmsg_mid targetTrs.
-    Local Definition targetSpecMid := svmMsgIdF extIdx1 extIdx2 targetMid.
-    Local Definition targetPrec: PreCond := ltac:(get_precond targetTrs).
+    Ltac get_precond trs pname :=
+      cbner (pmsg_precond trs) pname.
 
     Ltac mv_rewriter :=
       repeat
@@ -80,19 +95,16 @@ Section Impl.
         as Hnc by (cbn; intros; dest; intuition mv_rewriter);
       clear Hnc.
 
-    Ltac find_new_prec cprec invs :=
-      match invs with
+    Ltac find_new_prec cprec invs pname :=
+      let hcprec := (eval hnf in cprec) in
+      let hinvs := (eval hnf in invs) in
+      match hinvs with
       | nil => fail
       | ?inv :: ?invs' =>
-        tryif (inv_not_compatible cprec inv)
-        then (exact inv)
-        else find_new_prec cprec invs'
+        tryif (inv_not_compatible hcprec inv)
+        then (pose inv as pname)
+        else find_new_prec hcprec invs'
       end.
-
-    Local Definition newPrec: PreCond :=
-      ltac:(let tgt := (eval hnf in targetPrec) in
-            let invs := (eval hnf in svmImplChild1Inv) in
-            find_new_prec tgt invs).
 
     Ltac syn_step_init pimpl pimpl_ok :=
       econstructor;
@@ -102,7 +114,16 @@ Section Impl.
 
     Ltac syn_step_sim pimpl_ok :=
       apply simulation_pmsgs_added;
-      [apply pimpl_ok|].
+      [apply pimpl_ok|];
+      unfold Simulates; intros.
+
+    Ltac inv_step_seq :=
+      match goal with
+      | [H: step_seq _ _ _ _ |- _] => inv H
+      end.
+
+    Ltac simulates_silent :=
+      simpl; right; assumption.
 
     Definition synTrs:
       { impl1: System & SynthOk spec (SimTrs SvmR) svmP impl1 }.
@@ -112,7 +133,36 @@ Section Impl.
       - (* serializability *) admit.
       - (* simulation *)
         syn_step_sim impl0_ok.
-        unfold Simulates; intros.
+        inv_step_seq.
+
+        + (* silent *) simulates_silent.
+        + (* external message-in *)
+          (** TODO: Ltac simulates_lbl_in := (... below ...) *)
+          rewrite addPMsgsSys_isExternal, buildRawSys_isExternal in H1.
+          rewrite addPMsgsSys_isInternal, buildRawSys_isInternal in H2.
+          simpl; destruct sst1 as [soss1 smsgs1 sts].
+          eexists {| tst_oss := soss1;
+                     tst_msgs := distributeMsg (toTMsgU _) smsgs1;
+                     tst_tid := sts |}.
+          eexists (IlblIn (toTMsgU _)).
+          repeat split;
+            [|discriminate (* IlblIn _ <> emptyLabel *)
+             |assumption (* States don't change 
+                          * when external messages are added *)
+            ].
+          econstructor.
+          * pose proof (validMsgMap_from_isExternal _ _ _ svmMsgF_ValidMsgMap).
+            rewrite <-H0; auto.
+          * pose proof svmMsgF_ValidMsgMap.
+            specialize (H0 emsg); dest.
+            rewrite <-H3; auto.
+
+        + (* internal transaction started *)
+          admit.
+
+        + (* internal forwarding *)
+          admit.
+
     Admitted.
     
   End SynStep.
